chore: cleanup proofs and improve compile times

SP1Chips/JalChip.lean
@@ -1,4 +1,5 @@
 import SP1Operations.Operation.AddOperation
+import SP1Chips.Jal.Constraints
 
 namespace JalChip
 
@@ -6,85 +7,19 @@ open BitVec
 
 open Sail SailState BitVec LeanRV64IM.Functions
 
-def constraints (Main : Vector (Fin BB) 31) : SP1ConstraintList :=
-  let E0 : Fin BB := Main[30] - 1
-  let E1 : Fin BB := Main[30] * E0
-  let CS0 : SP1ConstraintList := AddOperation.constraints #v[Main[3], Main[4], Main[5], 0] #v[Main[14], Main[15], Main[16], Main[17]] { value := #v[Main[22], Main[23], Main[24], Main[25]] } Main[30]
-  let E2 : Fin BB := Main[1] * 65536
-  let E3 : Fin BB := Main[2] + E2
-  let E4 : Fin BB := Main[30] - 1
-  let E5 : Fin BB := Main[30] * E4
-  let E6 : Fin BB := E3 + 8
-  let E7 : Fin BB := Main[2] - 1
-  let E8 : Fin BB := E7 * 1761607681
-  let E9 : Fin BB := Main[30] - 1
-  let E10 : Fin BB := E9 * Main[13]
-  let E11 : Fin BB := Main[30] - Main[13]
-  let CS1 : SP1ConstraintList := AddOperation.constraints #v[Main[3], Main[4], Main[5], 0] #v[4, 0, 0, 0] { value := #v[Main[26], Main[27], Main[28], Main[29]] } E11
-  let E12 : Fin BB := Main[13] * Main[26]
-  let E13 : Fin BB := Main[13] * Main[27]
-  let E14 : Fin BB := Main[13] * Main[28]
-  let E15 : Fin BB := Main[1] * 65536
-  let E16 : Fin BB := Main[2] + E15
-  let E17 : Fin BB := Main[30] - 1
-  let E18 : Fin BB := Main[30] * E17
-  let E19 : Fin BB := Main[26] - 0
-  let E20 : Fin BB := Main[13] * E19
-  let E21 : Fin BB := Main[27] - 0
-  let E22 : Fin BB := Main[13] * E21
-  let E23 : Fin BB := Main[28] - 0
-  let E24 : Fin BB := Main[13] * E23
-  let E25 : Fin BB := Main[29] - 0
-  let E26 : Fin BB := Main[13] * E25
-  let E27 : Fin BB := E16 + 3
-  let E28 : Fin BB := Main[30] - 1
-  let E29 : Fin BB := Main[30] * E28
-  let E30 : Fin BB := E27 - Main[11]
-  let E31 : Fin BB := E30 - 1
-  let E32 : Fin BB := E31 - Main[12]
-  let E33 : Fin BB := E32 * 2013235201
-  [
-    (.assertZero E1),
-    (.assertZero Main[25]),
-    (.assertZero E5),
-    (.receive (.state Main[0] E3 Main[3] Main[4] Main[5]) Main[30]),
-    (.send (.state Main[0] E6 Main[22] Main[23] Main[24]) Main[30]),
-    (.send (.byte (ByteOpcode.ofNat 6) E8 13 0) Main[30]),
-    (.send (.byte (ByteOpcode.ofNat 3) 0 Main[1] 0) Main[30]),
-    (.assertZero E10),
-    (.assertZero Main[29]),
-    (.assertZero E12),
-    (.assertZero E13),
-    (.assertZero E14),
-    (.assertZero E18),
-    (.send (.program Main[3] Main[4] Main[5] (Opcode.ofNat 33) Main[6] Main[14] Main[15] Main[16] Main[17] Main[18] Main[19] Main[20] Main[21] Main[13] 1 1 111 0 0) Main[30]),
-    (.assertZero E20),
-    (.assertZero E22),
-    (.assertZero E24),
-    (.assertZero E26),
-    (.assertZero E29),
-    (.send (.byte (ByteOpcode.ofNat 6) Main[12] 16 0) Main[30]),
-    (.send (.byte (ByteOpcode.ofNat 3) 0 E33 0) Main[30]),
-    (.send (.memory Main[0] Main[11] Main[6] 0 0 Main[7] Main[8] Main[9] Main[10]) Main[30]),
-    (.receive (.memory Main[0] E27 Main[6] 0 0 Main[26] Main[27] Main[28] Main[29]) Main[30]),
-  ] ++ CS0 ++ CS1
-
-open LeanRV64IM.Functions
+variable (Main : Vector (Fin BB) 31) (s : SailState)
 
 lemma op_a_lt32_of_constraints {Main : Vector (Fin BB) 31}
-    (h_cstrs : (constraints Main).allHold)
-    (h_is_real : Main[30] = 1) : Main[6].val < 32 := by
+    (h_cstrs : (constraints Main).allHold) (h_is_real : Main[30] = 1) : Main[6].val < 32 := by
   simp only [BB_eq, Nat.reducePow]
   simp [SP1ConstraintList.allHold, constraints, SP1Constraint.toProp] at h_cstrs
-  have h : Main[6] < 32 := by aesop
-  clear h_cstrs
-  aesop
+  have h : Main[6] < 32 := by simp_all only [BB_eq, Fin.isValue, one_ne_zero, sub_self,
+    or_true, not_false_eq_true, forall_const, true_or, true_and]
+  simp_all only [BB_eq, Fin.isValue, gt_iff_lt]
+  exact h
 
-variable (Main : Vector (Fin BB) 31)
-  (s : SailState) (cstrs : (constraints Main).allHold)
-  (h_is_real : Main[30] = 1)
-
-def sp1_op_a : BitVec 5 := Main[6].val#'(op_a_lt32_of_constraints cstrs h_is_real)
+def sp1_op_a (cstrs : (constraints Main).allHold) (h_is_real : Main[30] = 1) : BitVec 5 :=
+  Main[6].val#'(op_a_lt32_of_constraints cstrs h_is_real)
 
 -- dt: could instead put `Word.toBitVec64 #v[Main[14], Main[15], Main[16], Main[17]]` here...
 def sp1_op_b : BitVec 21 := BitVec.ofNat 21 (Main[14].val + Main[15].val * 65536)
@@ -102,15 +37,14 @@ def spec_jal (imm : BitVec 21) (rd : regidx) : SailM Unit := do
 
 section move
 
-@[simp] -- common enough to want a lemma
-lemma Word.four_isU64 : Word.isU64 #v[4, 0, 0, 0] :=
-  Word.isU64_of_cases _ (by trivial) (by trivial) (by trivial) (by trivial)
+lemma BabyBear.val_mod4_eq_zero (x : Fin BB) : x.val % 4 = 0 ↔ x % 4 = 0 := by
+  rw [← Fin.val_inj]
+  simp only [BB_eq, Fin.isValue, Fin.mod_val, Fin.coe_ofNat_eq_mod, Nat.reduceMod, Nat.zero_mod]
 
 end move
 
 set_option debug.skipKernelTC true in
-set_option maxHeartbeats 0 in
-theorem SP1JAL_correct
+theorem SP1JAL_correct (cstrs : (constraints Main).allHold) (h_is_real : Main[30] = 1)
     (state_cstrs : (constraints Main).initialState s)
     (h_misa : Register.misa ∈ s.regs) :
     let op_a := sp1_op_a Main cstrs h_is_real
@@ -125,31 +59,25 @@ theorem SP1JAL_correct
   specialize h (by aesop)
 
   simp [SP1ConstraintList.allHold, constraints, SP1Constraint.toProp, sub_eq_zero,
-    h_is_real] at cstrs
+    h_is_real, Fin.isValue, BB_eq, true_and] at cstrs
 
   have h_sign_extend : Word.toBitVec64 #v[Main[14], Main[15], Main[16], Main[17]] =
       BitVec.signExtend 64 (BitVec.ofNat 21 (↑Main[14] + ↑Main[15] * 65536)) := by
-    have := cstrs.2.2.2.2.2.2.2.1.1.1
-    exact this
+    simp_all only
+
+  have hpc : BitVec.ofNat 64 (↑Main[3] + ↑Main[4] * 65536 + ↑Main[5] * 4294967296) =
+      Word.toBitVec64 #v[Main[3], Main[4], Main[5], 0] := by simp [Word.toBitVec64, Word.toNat]
 
   have hmod : (BitVec.ofNat 64 (↑Main[3] + ↑Main[4] * 65536 + ↑Main[5] * 4294967296) +
       Word.toBitVec64 #v[Main[14], Main[15], Main[16], Main[17]])[1] = false := by
     refine (mul4_means_0_1_are_0 ?_).2
-    have hpc : BitVec.ofNat 64 (↑Main[3] + ↑Main[4] * 65536 + ↑Main[5] * 4294967296) =
-      Word.toBitVec64 #v[Main[3], Main[4], Main[5], 0] := by simp [Word.toBitVec64, Word.toNat]
-    rw [hpc]
-    simp [Word.toBitVec64_add_mod_4, Word.add_toBitVec64_mod_4]
-    refine mul4_add_is_mul4 ?_ ?_
-    · simp
-      rw [ofNat64_mod_4_eq_zero_iff]
-      have : Main[3] % 4 = 0 := by aesop
-      clear cstrs
-      rw [Fin.mod_def] at this
-      rw [← Fin.val_inj] at this
-      simp at this
-      exact this
-    · simp
-      aesop
+
+    simp [hpc]
+    refine add_mod4_eq_zero_of_mod4_eq_zero ?_ ?_
+    · simp [ofNat_eq_ofNat, BabyBear.val_mod4_eq_zero]
+      simp_all only [BB_eq, Fin.isValue, true_and]
+    · simp only [ofNat_eq_ofNat, ofNat64_mod_4_eq_zero_iff]
+      simp_all only [BB_eq, Fin.isValue, true_and]
 
   simp [spec_jal, sp1_jal, execute_JAL, op_a, op_b, sp1_op_b, sp1_op_a]
 
@@ -157,40 +85,30 @@ theorem SP1JAL_correct
       #v[Main[3], Main[4], Main[5], 0]
       #v[Main[14], Main[15], Main[16], Main[17]]
       {value := #v[Main[22], Main[23], Main[24], Main[25]]} 1) := by
-    aesop
+    simp_all only [Fin.isValue, BB_eq, true_and]
+    simp_all only [Fin.isValue, _root_.and_self, and_true, true_and, or_true]
 
-  have pc_isU64 : Word.isU64 #v[Main[3], Main[4], Main[5], 0] := by
-    refine Word.isU64_of_cases _ ?_ ?_ ?_ (by simp)
-    · simp
-      aesop
-    · simp
-      aesop
-    · simp
-      aesop
-
+  have h3 : Main[3] < 65536 := by simp_all only
+  have h4 : Main[4] < 65536 := by simp_all only
+  have h5 : Main[5] < 65536 := by simp_all only
+  have h14 : Main[14] < 65536 := by simp_all only
+  have h15 : Main[15] < 65536 := by simp_all only
+  have h16 : Main[16] < 65536 := by simp_all only
+  have h17 : Main[17] < 65536 := by simp_all only
+  have pc_isU64 : Word.isU64 #v[Main[3], Main[4], Main[5], 0] :=
+    Word.isU64_of_cases _ h3 h4 h5 (by simp)
   have imm_isU64 : Word.isU64 #v[Main[14], Main[15], Main[16], Main[17]] := by
-    refine Word.isU64_of_cases _ ?_ ?_ ?_ ?_
-    · simp
-      aesop
-    · simp
-      aesop
-    · simp
-      aesop
-    · simp
-      aesop
+    refine Word.isU64_of_cases _ h14 h15 h16 h17
 
-  have := AddOperation.correct _ _ _  _ rfl h_add_imm
-  have h_add' := (this pc_isU64 imm_isU64).2
+  have h_add' := (AddOperation.correct _ _ _  _ rfl h_add_imm pc_isU64 imm_isU64).2
   simp [Word.toBitVec64, Word.toNat] at h_add'
 
   simp only [ext_control_check_pc, bit_to_bool, access, ofBool, bits_of_virtaddr, Nat.one_lt_ofNat,
     getElem!_pos, ofNat_eq_ofNat, currentlyEnabled, hartSupports, Bool.false_and, Bool.false_or,
     Bool.and_self, bind_pure_comp, Functor.map_map, bind_map_left, EStateM.run_bind,
-    run_bool_bit_backwards,
-    sign_extend, Sail.BitVec.signExtend, ← h_sign_extend]
+    run_bool_bit_backwards, sign_extend, Sail.BitVec.signExtend, ← h_sign_extend]
 
   have h13_is_bool : Main[13] = 0 ∨ Main[13] = 1 := by aesop
-
   have h6_lt : Main[6].val < 2^5 := by aesop
 
   cases h13_is_bool with
@@ -202,37 +120,28 @@ theorem SP1JAL_correct
         simp [← BitVec.toFin_inj] at h
         rw [← Fin.val_inj] at h
         simpa using h
-
-      rw [run_readReg, read_pc]
-      simp [h6]
+      specialize h6' h6_lt
+      rw [BitVec.ofNatLT_eq_ofNat] at h6'
+      rw [run_readReg]
+      simp [h6, read_pc]
       rw [run_readReg]
       simp [Std.ExtDHashMap.get?_insert, read_pc]
       simp [hmod]
       rw [run_readReg]
       simp [Std.ExtDHashMap.get?_insert, Std.ExtDHashMap.get?_eq_some_get h_misa]
       rw [run_readReg]
-
-      simp [h6']
-      have h6'' := h6' h6_lt
-      rw [BitVec.ofNatLT_eq_ofNat] at h6''
-      simp [h6'']
-      rw [h_add']
+      simp [BitVec.ofNatLT_eq_ofNat, h6', h_add']
       simp [Word.toBitVec64, Word.toNat]
       have h_add_pc : List.Forall SP1Constraint.toProp (AddOperation.constraints
-          #v[Main[3], Main[4], Main[5], 0]
-          #v[4, 0, 0, 0]
-          {value := #v[Main[26], Main[27], Main[28], Main[29]]} 1) := by
-        aesop
-      have := AddOperation.correct _ _ _  _ rfl h_add_pc
-      have h_add_pc' := (this pc_isU64 Word.four_isU64).2
+          #v[Main[3], Main[4], Main[5], 0] #v[4, 0, 0, 0]
+          {value := #v[Main[26], Main[27], Main[28], Main[29]]} 1) := by aesop
+      have h_add_pc' := (AddOperation.correct _ _ _  _ rfl h_add_pc pc_isU64 Word.four_isU64).2
       simp [Word.toBitVec64, Word.toNat] at h_add_pc'
-      rw [h_add_pc']
-      rw [BitVec.ofNatLT_eq_ofNat]
+      rw [h_add_pc', BitVec.ofNatLT_eq_ofNat]
 
   | inr h13_is_1 =>
       simp [h13_is_1] at cstrs
       have h6 : Main[6] = 0 := by aesop
-
       simp [h6]
       rw [run_readReg]
       simp [read_pc]
@@ -241,8 +150,7 @@ theorem SP1JAL_correct
       rw [run_readReg]
       simp [Std.ExtDHashMap.get?_insert, Std.ExtDHashMap.get?_eq_some_get h_misa]
       rw [run_readReg]
-      simp [h_add']
-      simp [Word.toBitVec64, Word.toNat]
+      simp [h_add', Word.toBitVec64, Word.toNat]
 
 end JalChip
 
